Working example of monad reduction
- Fixed bug in monad reduction
- Finished reification
- Fixed bug in reification of applications when the head
  symbol is a deBruijn index.
  - This solution could be much more general.
- Demo for monad reduction.
- reification for monad expressions.

examples/Monad2/MonadExpr.v
@@ -1,3 +1,4 @@
+Require Import ExtLib.Structures.Monad.
 Require Import MirrorCore.SymI.
 Require Import MirrorCore.SymEnv.
 Require Import MirrorCore.Lambda.Expr.
@@ -10,3 +11,29 @@ Set Strict Implicit.
 Definition mext : Type := (SymEnv.func + mfunc)%type.
 
 Definition mexpr := expr typ mext.
+
+Section mext.
+  Variable m : Type -> Type.
+  Variable Monad_m : Monad m.
+  Variable tys : types.
+  Let typD := typD m tys.
+  Variable fs : functions typD.
+
+  Instance RSym_mext : RSym typD mext.
+  apply RSym_sum.
+  eapply SymEnv.RSym_func. apply fs.
+  apply RSym_mfunc. assumption.
+  Defined.
+
+  Definition exprD (ts : list Type) (us vs : EnvI.env typD) (t : typ) (e : mexpr) : option (typD ts t) :=
+    let (tus,us) := EnvI.split_env us in
+    let (tvs,vs) := EnvI.split_env vs in
+    match @ExprDenote.exprD' typ typD mext
+                             (RType_typ _ _) _ RSym_mext
+                             ts tus tvs t e
+    with
+      | None => None
+      | Some val => Some (val us vs)
+    end.
+
+End mext.
